pulse/examples/steel/Selectors.Tree.Core.fsti
@@ -2,6 +2,7 @@ module Selectors.Tree.Core
 
 open Steel.Memory
 open Steel.SelEffect
+open Steel.SelReference
 
 module Spec = Trees
 
